physical/config.mk
@@ -1,10 +1,10 @@
 PROJECT_ROOT := $(shell git rev-parse --show-toplevel)
 
 # Physical Design Configuration
-export DESIGN_NAME = RV32IDecoder
+export DESIGN_NAME = RV32IMDecoder
 export PLATFORM    = asap7
 
-export VERILOG_FILES = $(PROJECT_ROOT)/output/sv-from-lean/RV32IDecoder.sv
+export VERILOG_FILES = $(PROJECT_ROOT)/output/sv-from-lean/RV32IMDecoder.sv
 export SDC_FILE      = $(PROJECT_ROOT)/physical/constraints.sdc
 
 # Timing Target
